Hashmap/DHashMap/Lemmas.lean
@@ -19,7 +19,104 @@ theorem List.perm_append_comm_assoc (l₁ l₂ l₃ : List α) : l₁ ++ (l₂ +
 
 namespace MyLean.DHashMap
 
+-- TODO: this is just about arrays
+theorem Array.exists_of_update (self : Array (AssocList α β)) (i d h) :
+    ∃ l₁ l₂, self.data = l₁ ++ self[i] :: l₂ ∧ List.length l₁ = i.toNat ∧
+      (self.uset i d h).data = l₁ ++ d :: l₂ := by
+  simp [Array.getElem_eq_data_get]; exact List.exists_of_set' _
+
+-- TODO
+theorem List.length_le_append_right {l₁ l₂ : List α} : l₁.length ≤ (l₁ ++ l₂).length := by
+  simpa using Nat.le_add_right _ _
+
+-- TODO
+theorem List.length_le_append_left {l₁ l₂ : List α} : l₂.length ≤ (l₁ ++ l₂).length := by
+  simpa using Nat.le_add_left _ _
+
+-- TODO
+theorem List.get_eq_get_append_right {l₁ : List α} (l₂ : List α) {n : Fin l₁.length} :
+    l₁.get n = (l₁ ++ l₂).get (n.castLE length_le_append_right) := by
+  rw [get_append]; rfl
+
+-- TODO
+theorem List.get_eq_get_append_left (l₁ : List α) {l₂ : List α} {n : Fin l₂.length} :
+    l₂.get n = (l₁ ++ l₂).get ((n.addNat l₁.length).cast (by simp [Nat.add_comm l₂.length])) := by
+  rw [get_append_right]
+  · simp
+  · simpa using Nat.le_add_left _ _
+  · simp
+
+-- TODO
+theorem List.get_eq_get_cons (a : α) {l : List α} {n : Fin l.length} :
+    l.get n = (a :: l).get ((n.addNat 1).cast (by simp)) := by
+  erw [get_cons_succ]
+
+-- TODO
+theorem List.get_congr {l₁ l₂ : List α} {n : Fin l₁.length} (h : l₁ = l₂) :
+    l₁.get n = l₂.get (n.cast (h ▸ rfl)) := by
+  cases h; rfl
+
+-- TODO
+theorem Nat.lt_of_eq_of_lt {n m k : Nat} : n = m → m < k → n < k :=
+  fun h₁ h₂ => h₁ ▸ h₂
+
+theorem exists_bucket_of_uset [BEq α] [Hashable α]
+  (self : Array (AssocList α β)) (i : USize) (hi : i.toNat < self.size) (d : AssocList α β) :
+    ∃ l, self.data.bind AssocList.toList ~ self[i.toNat].toList ++ l ∧
+      (self.uset i d hi).data.bind AssocList.toList ~ d.toList ++ l ∧
+      (∀ [EquivBEq α] [LawfulHashable α],
+        IsHashSelf self → ∀ k : α, ((hash k).toUSize % self.size).toNat = i.toNat → l.containsKey k = false) := by
+  obtain ⟨l₁, l₂, h₁, h₂, h₃⟩ := Array.exists_of_update self i d hi
+  refine ⟨l₁.bind AssocList.toList ++ l₂.bind AssocList.toList, ?_, ?_, ?_⟩
+  · rw [h₁]
+    simpa using List.perm_append_comm_assoc _ _ _
+  · rw [h₃]
+    simpa using List.perm_append_comm_assoc _ _ _
+  · intro _ _ h k
+    rw [← Decidable.not_imp_not]
+    intro hk
+    simp only [Bool.not_eq_false, containsKey_eq_true_iff_exists_mem, mem_append, mem_bind] at hk
+    obtain ⟨⟨k', v'⟩, ⟨(⟨a, ha₁, ha₂⟩|⟨a, ha₁, ha₂⟩), hk⟩⟩ := hk
+    · obtain ⟨n, hn⟩ := List.get_of_mem ha₁
+      rw [List.get_eq_get_append_right (self[i] :: l₂)] at hn
+      suffices ((hash k').toUSize % self.size).toNat = n from
+        Nat.ne_of_lt (Nat.lt_of_eq_of_lt (hash_eq hk ▸ this) (h₂ ▸ n.2))
+      rw [List.get_congr h₁.symm, ← Array.getElem_eq_data_get] at hn
+      exact (h.hashes_to n (by omega)).hash_self _ (hn.symm ▸ ha₂)
+    · obtain ⟨n, hn⟩ := List.get_of_mem ha₁
+      rw [List.get_eq_get_cons self[i], List.get_eq_get_append_left l₁] at hn
+      suffices ((hash k').toUSize % self.size).toNat = n + 1 + l₁.length from
+        Nat.ne_of_lt' (h₂ ▸ ((hash_eq hk ▸ this) ▸ by omega))
+      rw [List.get_congr h₁.symm, ← Array.getElem_eq_data_get] at hn
+      refine (h.hashes_to (n + 1 + l₁.length) ?_).hash_self _ (hn.symm ▸ ha₂)
+      rw [Array.size_eq_length_data, h₁, length_append, length_cons]
+      omega
+
+theorem exists_bucket [BEq α] [Hashable α]
+    (self : Array (AssocList α β)) (i : USize) (hi : i.toNat < self.size) :
+      ∃ l, self.data.bind AssocList.toList ~ self[i.toNat].toList ++ l ∧
+        (∀ [EquivBEq α] [LawfulHashable α], IsHashSelf self → ∀ k,
+          ((hash k).toUSize % self.size).toNat = i.toNat → l.containsKey k = false) := by
+  obtain ⟨l, h₁, -, h₂⟩ := exists_bucket_of_uset self i hi .nil
+  exact ⟨l, h₁, h₂⟩
+
 namespace Raw
+
+@[simp]
+theorem toList_empty {c} : (empty c : Raw α β).toList = [] := by
+  suffices ∀ d, (List.replicate d AssocList.nil).bind AssocList.toList = [] from this _
+  intro d
+  induction d <;> simp_all
+
+theorem findEntry?WellFormed_eq_findEntry_toList [BEq α] [EquivBEq α] [Hashable α] [LawfulHashable α]
+    (m : { m : Raw α β // 0 < m.buckets.size }) (h : m.1.WF) (a : α) :
+      Raw.findEntry?WellFormed m a = m.1.toList.findEntry? a := by
+  rw [findEntry?WellFormed]
+  dsimp only [Array.ugetElem_eq_getElem]
+  obtain ⟨l, hl, hlk⟩ := exists_bucket m.1.buckets (mkIdx (hash a) m.2).1 (mkIdx (hash a) m.2).2
+  refine Eq.trans ?_ (List.findEntry?_of_perm (WF_of_perm hl.symm h.distinct) hl.symm)
+  rw [AssocList.findEntry?_eq, findEntry?_append_of_containsKey_eq_false]
+  exact hlk h.buckets_hash_self _ rfl
 
 end Raw
 
